add not-volatile-condition on AsmC

x86/AsmgenproofC0.v
@@ -28,35 +28,51 @@ Require Import MachC Mach.
 Require Import Asm.
 Require Import Asmgen.
 Require Import Conventions.
-Require Import sflib Asmgenproof0.
+Require Import sflib Asmgenproof0 Skeleton.
 
 (** * Processor registers and register states *)
 
 Section MATCH_STACK.
 
+Variable ske: SkEnv.t.
+
+Inductive not_volatile: val -> Prop :=
+| not_volatile_intro
+    blk ofs
+    (NOTVOL: Senv.block_is_volatile ske blk = false)
+  :
+    not_volatile (Vptr blk ofs true)
+.
+
 Variable ge: Mach.genv.
+
 Variable initial_parent_sp : val.
-Hypothesis initial_parent_sp_def : initial_parent_sp <> Vundef.
+Hypothesis initial_parent_sp_not_volatile : not_volatile (initial_parent_sp).
 Variable initial_parent_ra : val.
 Hypothesis initial_parent_ra_ptr : Val.has_type initial_parent_ra Tptr.
 Hypothesis initial_parent_ra_fake : ~ ValuesC.is_real_ptr initial_parent_ra.
 
 Inductive match_stack: list Mach.stackframe -> Prop :=
-  | match_stack_dummy
-    :
-      match_stack ((dummy_stack initial_parent_sp initial_parent_ra)::[])
-  | match_stack_cons: forall fb sp ra c s f tf tc,
-      Genv.find_funct_ptr ge fb = Some (Internal f) ->
-      transl_code_at_pc ge ra fb f c false tf tc ->
-      sp <> Vundef ->
-      match_stack s ->
+| match_stack_dummy
+  :
+    match_stack ((dummy_stack initial_parent_sp initial_parent_ra)::[])
+| match_stack_cons: forall fb sp ra c s f tf tc,
+    Genv.find_funct_ptr ge fb = Some (Internal f) ->
+    transl_code_at_pc ge ra fb f c false tf tc ->
+    not_volatile sp ->
+    (* sp <> Vundef -> *)
+    match_stack s ->
+    (* forall (NOTVOL: not_volatile sp), *)
       match_stack (Stackframe fb sp ra c :: s).
+
+Lemma parent_sp_not_volatile: forall s, match_stack s -> not_volatile (parent_sp s).
+Proof.
+  induction 1; auto.
+Qed.
 
 Lemma parent_sp_def: forall s, match_stack s -> parent_sp s <> Vundef.
 Proof.
-  induction 1; simpl.
-  unfold Vnullptr; destruct Archi.ptr64; congruence.
-  auto.
+  intros s MATCH. destruct (parent_sp_not_volatile _ MATCH). ss.
 Qed.
 
 Lemma lessdef_parent_sp:
